theories/base_logic/lib/fupd_level.v
@@ -8,12 +8,119 @@ Set Default Proof Using "Type".
 Export invG.
 Import uPred.
 
-Definition AE' (n: nat) : coPset := (↑(nroot.@(1%positive).@(n))).
-Fixpoint AE_def (n: nat) :=
+
+(* We start by constructing a way to divide up a namespace into a countably infinite sequence of name spaces with *)
+
+Fixpoint ndc (N: namespace) (n: nat) : namespace :=
+  match n with
+  | O => N
+  | S n' => ndc (N.@(1%positive)) n'
+  end.
+
+Lemma ndc_tail N n :
+  ndc N (S n) = (ndc N n).@(1%positive).
+Proof. revert N. induction n => N; first done. rewrite -IHn => //=. Qed.
+
+Definition nomega (N: namespace) (mn: option nat) : coPset :=
+  match mn with
+  | None => ↑(N.@(2%positive))
+  | Some n => ↑(ndc (N.@(1%positive)) n) ∪ ↑(N.@(2%positive))
+  end.
+
+Lemma ndc_anti_mono N n1 n2:
+  n1 ≤ n2 →
+  (↑(ndc N n2) : coPset) ⊆ ↑(ndc N n1).
+Proof.
+  induction 1.
+  - reflexivity.
+  - transitivity (↑(ndc N m) : coPset); last auto.
+    clear. revert N. induction m => N.
+    * rewrite //=. solve_ndisj.
+    * rewrite ndc_tail. solve_ndisj.
+Qed.
+
+Lemma ndc_subset_root N n:
+  (↑ (ndc N n) : coPset) ⊆ ↑N.
+Proof.
+  induction n. solve_ndisj. etransitivity; last eauto.
+  apply ndc_anti_mono; eauto.
+Qed.
+
+Definition ndc_S_diff N n : coPset := (↑ (ndc N n)) ∖ (↑ (ndc N (S n))).
+
+Lemma ndc_compl_S_inf N n: ¬ set_finite (ndc_S_diff N n).
+Proof.
+  rewrite /ndc_S_diff.
+  match goal with
+  | [ |- ¬ set_finite ?X ] => cut ((↑ndc N n.@(2%positive)) ⊆ X)
+  end.
+  { pose proof (nclose_infinite (ndc N n.@(2%positive))) as Hinf. intros => Hfalse.
+    apply Hinf. eapply set_finite_subseteq; eauto. }
+  rewrite ndc_tail. solve_ndisj.
+Qed.
+
+Lemma nomega_anti_mono_Some N n1 n2:
+  n1 ≤ n2 →
+  nomega N (Some n2) ⊆ nomega N (Some n1).
+Proof. intros Hle => //=.  pose proof (ndc_anti_mono (N.@1%positive) n1 n2). set_solver. Qed.
+
+Lemma nomega_anti_mono_None N n:
+  nomega N None ⊆ nomega N (Some n).
+Proof. rewrite //=. set_solver. Qed.
+
+Definition omega_le (mj1 mj2: option nat) : Prop :=
+  match mj1, mj2 with
+  | None, _ => True
+  | Some n1, Some n2 => n2 ≤ n1
+  | _, _ => False
+  end.
+
+Lemma nomega_omege_le N mj1 mj2 :
+  omega_le mj1 mj2 →
+  nomega N mj1 ⊆ nomega N mj2.
+Proof.
+  destruct mj1, mj2; try (inversion 1; done).
+  - apply nomega_anti_mono_Some.
+  - intros _. apply nomega_anti_mono_None.
+Qed.
+
+Lemma nomega_subset_root N mj :
+  nomega N mj ⊆ ↑ N.
+Proof.
+  destruct mj => //=.
+  - apply union_least.
+    * etransitivity; first eapply ndc_subset_root. solve_ndisj.
+    * solve_ndisj.
+  - solve_ndisj.
+Qed.
+
+(*
+Fixpoint slice_string (j: nat) : namespace :=
+  match j with
+  | O => nroot
+  | S n' => nroot.@(1%positive).@(slice_string n')
+  end.
+*)
+
+Definition AE'_ns (n : nat) : namespace := nroot.@(1%positive).@(n).
+Definition AE' (n: nat) : coPset := ↑(AE'_ns n).
+Definition AE'' (n: nat) mj := nomega (AE'_ns n) mj.
+
+Fixpoint AE_full_def (n: nat) :=
   AE' n ∪
   match n with
   | O => ∅
-  | S n' => AE_def n'
+  | S n' => AE_full_def n'
+  end.
+Definition AE_full_aux : seal AE_full_def. Proof. by eexists. Qed.
+Definition AE_full := AE_full_aux.(unseal).
+Definition AE_full_eq : AE_full = AE_full_def :=
+  AE_full_aux.(seal_eq).
+
+Definition AE_def (n: nat) (mj: option nat) :=
+  match n with
+  | O => ∅
+  | S n' => AE'' n mj ∪ AE_full n'
   end.
 Definition AE_aux : seal AE_def. Proof. by eexists. Qed.
 Definition AE := AE_aux.(unseal).
@@ -29,9 +136,9 @@ Qed.
 
 Lemma AE'_disj n1 n2 : n1 ≠ n2 → AE' n1 ## AE' n2.
 Proof. solve_ndisj. Qed.
-Lemma AE'_disj_AE n1 n2 : n1 < n2 → AE' n2 ## AE n1.
+Lemma AE'_disj_AE_full n1 n2 : n1 < n2 → AE' n2 ## AE_full n1.
 Proof.
-  revert n2. rewrite AE_eq.
+  revert n2. rewrite AE_full_eq.
   induction n1 => n2 Hlt.
   - rewrite //= right_id. apply AE'_disj. lia.
   - rewrite //=.
@@ -39,43 +146,188 @@ Proof.
     feed pose proof (AE'_disj n2 (S n1)); first lia.
     set_solver.
 Qed.
-Lemma AE_mono n1 n2 : n1 ≤ n2 → AE n1 ⊆ AE n2.
-Proof. rewrite AE_eq. induction 1; rewrite //=; set_solver. Qed.
+Lemma AE_full_mono n1 n2 : n1 ≤ n2 → AE_full n1 ⊆ AE_full n2.
+Proof. rewrite AE_full_eq. induction 1; rewrite //=; set_solver. Qed.
 Lemma AE'_subset_AlwaysEn n : AE' n ⊆ AlwaysEn.
 Proof. rewrite AlwaysEn_alt. solve_ndisj. Qed.
-Lemma AE_subset_AlwaysEn n : AE n ⊆ AlwaysEn.
-Proof. rewrite AE_eq AlwaysEn_alt; induction n; solve_ndisj. Qed.
-Lemma AE_MaybeEn_disj n E : AE n ## MaybeEn E.
+Lemma AE_full_subset_AlwaysEn n : AE_full n ⊆ AlwaysEn.
+Proof. rewrite AE_full_eq AlwaysEn_alt. induction n; solve_ndisj. Qed.
+Lemma AE_full_MaybeEn_disj n E : AE_full n ## MaybeEn E.
 Proof.
-  pose proof (AE_subset_AlwaysEn n).
+  pose proof (AE_full_subset_AlwaysEn n).
   cut (AlwaysEn ## MaybeEn E); last by apply coPset_inl_inr_disj.
   { set_solver. }
 Qed.
+Lemma AE''_subset_AE' n mj : AE'' n mj ⊆ AE' n.
+Proof. rewrite /AE''/AE'. apply nomega_subset_root. Qed.
+Lemma AE''_disj_AE_full n1 n2 mj : n1 < n2 → AE'' n2 mj ## AE_full n1.
+Proof.
+  pose proof (AE''_subset_AE' n2 mj).
+  pose proof (AE'_disj_AE_full n1 n2). intros.
+  set_solver.
+Qed.
+Lemma AE_subset_AE_full n mj : AE n mj ⊆ AE_full n.
+Proof.
+  rewrite AE_eq AE_full_eq /AE_def /AE_full_def -/AE_full_def.
+  destruct n; simpl; try set_solver.
+  apply union_least.
+  * etransitivity; last eapply union_subseteq_l. apply AE''_subset_AE'.
+  * rewrite AE_full_eq; set_solver.
+Qed.
+Lemma AE_subset_le_AE_full n1 n2 mj : n1 ≤ n2 → AE n1 mj ⊆ AE_full n2.
+Proof.
+  induction 1.
+  - apply AE_subset_AE_full.
+  - rewrite AE_full_eq /AE_full_def -/AE_full_def -AE_full_eq.
+    set_solver.
+Qed.
+Lemma AE_full_lt_subset_AE n1 n2 mj : n1 < n2 → AE_full n1 ⊆ AE n2 mj.
+Proof.
+  induction 1.
+  * rewrite AE_eq /AE_def. set_solver.
+  * rewrite AE_eq /AE_def. etransitivity; last eapply union_subseteq_r.
+    apply AE_full_mono; eauto. lia.
+Qed.
 
-Opaque AE.
+Lemma difference_union_same_L (X Y Z : coPset):
+  X ## Z → Y ## Z →
+  (X ∪ Z) ∖ (Y ∪ Z) = X ∖ Y.
+Proof. set_solver. Qed.
 
-Local Hint Extern 0 (AE _ ## MaybeEn _) => apply AE_MaybeEn_disj : core.
+Lemma disjoint_subseteq (X Y Z : coPset):
+  X ⊆ Y →
+  Y ## Z →
+  X ## Z.
+Proof. set_solver. Qed.
+
+Lemma AE'_disj_lt_AE n1 mj n2 : n1 < n2 → AE n1 mj ## AE' n2.
+Proof.
+  intros Hlt.
+  eapply disjoint_subseteq.
+  { eapply AE_subset_AE_full. }
+  symmetry. by apply AE'_disj_AE_full.
+Qed.
+
+Lemma AE_subset_mono n1 n2 mj1 mj2 :
+  (n1 < n2 ∨ (n1 = n2 ∧ omega_le mj1 mj2)) →
+  AE n1 mj1 ⊆ AE n2 mj2.
+Proof.
+  intros [Hlt|Heq].
+  - induction Hlt.
+    * rewrite AE_eq /= -AE_eq. etransitivity; last eapply union_subseteq_r.
+      apply AE_subset_AE_full.
+    * transitivity (AE_full m).
+      ** apply AE_subset_le_AE_full; lia.
+      ** apply AE_full_lt_subset_AE. lia.
+  - destruct Heq as (->&Hle).
+    rewrite AE_eq /AE_def; destruct n2; first set_solver+.
+    rewrite /AE''. apply union_mono_r. by apply nomega_omege_le.
+Qed.
+
+Lemma AE_subset_AlwaysEn n mj : AE n mj ⊆ AlwaysEn.
+Proof.
+  etransitivity; first eapply (AE_subset_le_AE_full n n mj); auto.
+  apply AE_full_subset_AlwaysEn.
+Qed.
+
+Lemma AE_MaybeEn_disj n mj E : AE n mj ## MaybeEn E.
+Proof.
+  pose proof (AE_full_MaybeEn_disj n E).
+  pose proof (AE_subset_AE_full n mj). set_solver.
+Qed.
+
+Definition AE_next n mj : coPset :=
+  match mj with
+  | Some j => AE n (Some (S j))
+  | None =>
+    match n with
+    | O => ∅
+    | S n => AE n (Some O)
+    end
+  end.
+
+
+Definition AE_S_diff n j : coPset :=
+  AE n (Some j) ∖ AE n (Some (S j)).
+
+Definition AE_next_diff n mj : coPset := AE n mj ∖ AE_next n mj.
+
+Lemma AE_S_diff_inf n j: ¬ set_finite (AE_S_diff (S n) j).
+Proof.
+  rewrite /AE_S_diff.
+  rewrite AE_eq /AE_def.
+  rewrite difference_union_same_L; swap 1 3.
+  { eapply AE''_disj_AE_full; lia. }
+  { eapply AE''_disj_AE_full; lia. }
+  rewrite /=.
+  rewrite difference_union_same_L; swap 1 3.
+  { match goal with
+      | [ |- ↑ (ndc ?X ?j) ## _] => pose proof (ndc_subset_root X j)
+    end. eapply disjoint_subseteq; first eassumption.
+    solve_ndisj. }
+  { match goal with
+      | [ |- ↑ (ndc ?X ?j) ## _] => pose proof (ndc_subset_root X j)
+    end. eapply disjoint_subseteq; first eassumption.
+    solve_ndisj. }
+  apply ndc_compl_S_inf.
+Qed.
+
+Lemma AE_next_diff_inf n mj: ¬ set_finite (AE_next_diff (S n) mj).
+Proof.
+  destruct mj; first apply AE_S_diff_inf.
+  rewrite /=. rewrite /AE_next_diff/AE_next. rewrite AE_eq /=.
+  match goal with
+    | [ |- ¬ set_finite ?X ] => assert (↑ (AE'_ns (S n).@2%positive) ⊆ X)
+  end.
+  { cut (↑AE'_ns (S n).@2%positive ## AE_def n (Some 0)).
+    { set_solver. }
+    eapply (disjoint_subseteq _ (AE' (S n))).
+    { rewrite /AE'. solve_ndisj. }
+    rewrite -AE_eq. symmetry. eapply AE'_disj_lt_AE. lia.
+  }
+  intros Hfin. eapply set_finite_subseteq in Hfin; last eassumption.
+  eapply nclose_infinite; eauto.
+Qed.
+
+Local Hint Extern 0 (AE_full _ ## MaybeEn _) => apply AE_full_MaybeEn_disj : core.
+Local Hint Extern 0 (AE _ _ ## MaybeEn _) => apply AE_MaybeEn_disj : core.
 Local Hint Extern 0 (AlwaysEn ## MaybeEn _) => apply coPset_inl_inr_disj : core.
 
+Definition uPred_fupd_split_level_def `{!invG Σ} (E1 E2 : coPset) (k : nat) mj (P : iProp Σ) : iProp Σ :=
+  wsat (S k) ∗ ownE (AE (S k) mj ∪ MaybeEn E1) ==∗ ◇ (wsat (S k) ∗ ownE (AE (S k) mj ∪ MaybeEn E2) ∗ P).
+Definition uPred_fupd_split_level_aux `{!invG Σ} : seal uPred_fupd_split_level_def. Proof. by eexists. Qed.
+Definition uPred_fupd_split_level `{!invG Σ} := uPred_fupd_split_level_aux.(unseal).
+Definition uPred_fupd_split_level_eq `{!invG Σ} : uPred_fupd_split_level = uPred_fupd_split_level_def :=
+  uPred_fupd_split_level_aux.(seal_eq).
+
 Definition uPred_fupd_level_def `{!invG Σ} (E1 E2 : coPset) (k : nat) (P : iProp Σ) : iProp Σ :=
-  wsat (S k) ∗ ownE (AE (S k) ∪ MaybeEn E1) ==∗ ◇ (wsat (S k) ∗ ownE (AE (S k) ∪ MaybeEn E2) ∗ P).
+  uPred_fupd_split_level E1 E2 k None P.
 Definition uPred_fupd_level_aux `{!invG Σ} : seal uPred_fupd_level_def. Proof. by eexists. Qed.
 Definition uPred_fupd_level `{!invG Σ} := uPred_fupd_level_aux.(unseal).
 Definition uPred_fupd_level_eq `{!invG Σ} : uPred_fupd_level = uPred_fupd_level_def :=
   uPred_fupd_level_aux.(seal_eq).
 
+Reserved Notation "| k , j ={ E1 }=> Q"
+  (at level 99, E1, k at level 50, j at level 50, Q at level 200,
+   format "| k , j ={ E1 }=>  Q").
+Reserved Notation "| k , j ={ E1 , E2 }=> Q"
+  (at level 99, E1, E2, k at level 50, j at level 50, Q at level 200,
+   format "| k , j ={ E1 , E2 }=>  Q").
 Reserved Notation "| k ={ E1 }=> Q"
   (at level 99, E1, k at level 50, Q at level 200,
    format "| k ={ E1 }=>  Q").
 Reserved Notation "| k ={ E1 , E2 }=> Q"
   (at level 99, E1, E2, k at level 50, Q at level 200,
    format "| k ={ E1 , E2 }=>  Q").
+
 (*
 Reserved Notation "P = k ={ E1 , E2 }=∗ Q"
   (at level 99, E1,E2, k at level 50, Q at level 200,
    format "'[' P  '/' = k ={ E1 , E2 }=∗  Q ']'").
 *)
 
+Notation "| k , j ={ E1 , E2 }=> Q" := (uPred_fupd_split_level E1 E2 k j Q) : bi_scope.
+Notation "| k , j ={ E1 }=> Q" := (uPred_fupd_split_level E1 E1 k j Q) : bi_scope.
 Notation "| k ={ E1 , E2 }=> Q" := (uPred_fupd_level E1 E2 k Q) : bi_scope.
 Notation "| k ={ E1 }=> Q" := (uPred_fupd_level E1 E1 k Q) : bi_scope.
 (*
@@ -87,53 +339,73 @@ Section fupd_level.
 Context `{!invG Σ}.
 Implicit Types P: iProp Σ.
 Implicit Types E : coPset.
-Implicit Types k : nat.
+Implicit Types j k : nat.
+Implicit Types mj : option nat.
 
+Global Instance fupd_split_level_ne E1 E2 k: NonExpansive (uPred_fupd_split_level E1 E2 k mj).
+Proof. rewrite uPred_fupd_split_level_eq. solve_proper. Qed.
 Global Instance fupd_level_ne E1 E2 k: NonExpansive (uPred_fupd_level E1 E2 k).
 Proof. rewrite uPred_fupd_level_eq. solve_proper. Qed.
 
-Lemma fupd_level_intro_mask E1 E2 k P : E2 ⊆ E1 → P ⊢ |k={E1,E2}=> |k={E2,E1}=> P.
+Lemma fupd_split_level_intro_mask E1 E2 k mj P : E2 ⊆ E1 → P ⊢ |k,mj={E1,E2}=> |k,mj={E2,E1}=> P.
 Proof.
   intros (E1''&->&?)%subseteq_disjoint_union_L.
-  rewrite uPred_fupd_level_eq /uPred_fupd_level_def ?ownE_op // ?ownE_op_MaybeEn //.
+  rewrite uPred_fupd_split_level_eq /uPred_fupd_split_level_def ?ownE_op // ?ownE_op_MaybeEn //.
   by iIntros "$ ($ & $ & $ & HE) !> !> [$ [$ $]] !> !>" .
 Qed.
 
-Lemma except_0_fupd_level E1 E2 k P : ◇ (|k={E1,E2}=> P) ⊢ |k={E1,E2}=> P.
+Lemma fupd_level_intro_mask E1 E2 k P : E2 ⊆ E1 → P ⊢ |k={E1,E2}=> |k={E2,E1}=> P.
+Proof. rewrite uPred_fupd_level_eq; apply fupd_split_level_intro_mask. Qed.
+
+Lemma except_0_fupd_split_level E1 E2 k mj P : ◇ (|k,mj={E1,E2}=> P) ⊢ |k,mj={E1,E2}=> P.
 Proof.
-  rewrite uPred_fupd_level_eq /uPred_fupd_level_def.
+  rewrite uPred_fupd_split_level_eq /uPred_fupd_split_level_def.
   iIntros ">H [Hw HE]". iApply "H"; by iFrame.
 Qed.
 
+Lemma except_0_fupd_level E1 E2 k P : ◇ (|k={E1,E2}=> P) ⊢ |k={E1,E2}=> P.
+Proof. rewrite uPred_fupd_level_eq; apply except_0_fupd_split_level. Qed.
+
+Lemma fupd_split_level_mono E1 E2 k mj P Q : (P ⊢ Q) → (|k,mj={E1,E2}=> P) ⊢ |k,mj={E1,E2}=> Q.
+Proof.
+  rewrite uPred_fupd_split_level_eq. iIntros (HPQ) "HP HwE". rewrite -HPQ. by iApply "HP".
+Qed.
+
 Lemma fupd_level_mono E1 E2 k P Q : (P ⊢ Q) → (|k={E1,E2}=> P) ⊢ |k={E1,E2}=> Q.
-Proof.
-  rewrite uPred_fupd_level_eq. iIntros (HPQ) "HP HwE". rewrite -HPQ. by iApply "HP".
-Qed.
+Proof. rewrite uPred_fupd_level_eq; apply fupd_split_level_mono. Qed.
 
-Lemma ownE_AE_split_current_rest k :
-  ownE (AE (S k)) ⊣⊢  ownE (AE' (S k)) ∗ ownE (AE k).
+Lemma ownE_AE_split_current_rest k mj :
+  ownE (AE (S k) mj) ⊣⊢  ownE (AE_next_diff (S k) mj) ∗ ownE (AE_next (S k) mj).
 Proof.
-  rewrite {1}AE_eq /AE_def -/AE_def -AE_eq ownE_op //.
-  apply AE'_disj_AE; lia.
+  rewrite /AE_next_diff/AE_next.
+  rewrite -ownE_op. f_equiv.
+  {
+    rewrite difference_union_L.
+    rewrite (comm_L (∪)) subseteq_union_1_L //.
+    destruct mj; apply AE_subset_mono; naive_solver lia.
+  }
+  set_solver.
 Qed.
-Lemma ownE_AE_le_acc k1 k2 :
-  k1 ≤ k2 →
-  ownE (AE k2) -∗ ownE (AE k1) ∗ (ownE (AE k1) -∗ ownE (AE k2)).
-Proof. iIntros (?). iApply ownE_mono_le_acc. by apply AE_mono. Qed.
+Lemma ownE_AE_le_acc n1 mj1 n2 mj2 :
+  (n1 < n2 ∨ (n1 = n2 ∧ omega_le mj1 mj2)) →
+  ownE (AE n2 mj2) -∗ ownE (AE n1 mj1) ∗ (ownE (AE n1 mj1) -∗ ownE (AE n2 mj2)).
+Proof. iIntros (?). iApply ownE_mono_le_acc. by apply AE_subset_mono. Qed.
 
-Lemma ownE_AlwaysEn_le_acc k :
-  ownE (AlwaysEn) -∗ ownE (AE k) ∗ (ownE (AE k) -∗ ownE AlwaysEn).
+Lemma ownE_AlwaysEn_le_acc n1 mj1 :
+  ownE (AlwaysEn) -∗ ownE (AE n1 mj1) ∗ (ownE (AE n1 mj1) -∗ ownE AlwaysEn).
 Proof. iApply ownE_mono_le_acc. by apply AE_subset_AlwaysEn. Qed.
 
-Lemma fupd_level_le E1 E2 k1 k2 P : k1 ≤ k2 → (|k1={E1,E2}=> P) ⊢ |k2={E1,E2}=> P.
+Lemma fupd_split_level_le E1 E2 k1 k2 mj1 mj2 P :
+  (k1 < k2 ∨ (k1 = k2 ∧ omega_le mj1 mj2)) →
+  (|k1,mj1={E1,E2}=> P) ⊢ |k2,mj2={E1,E2}=> P.
 Proof.
-  rewrite ?uPred_fupd_level_eq /uPred_fupd_level_def.
+  rewrite ?uPred_fupd_split_level_eq /uPred_fupd_split_level_def.
   rewrite ?ownE_op //.
   iIntros (Hle) "HP (Hw&HAE&HE)".
   iDestruct (wsat_le_acc (S k1) (S k2) with "Hw") as "(Hw&Hclo)".
   { lia. }
-  iDestruct (ownE_AE_le_acc (S k1) (S k2) with "HAE") as "(HAE&Hclo')".
-  { lia. }
+  iDestruct (ownE_AE_le_acc (S k1) mj1 (S k2) mj2 with "HAE") as "(HAE&Hclo')".
+  { naive_solver lia. }
   iMod ("HP" with "[$]") as "H". iModIntro.
   iMod "H" as "(Hw&(HAE&HE)&HP)". iFrame.
   iModIntro.
@@ -141,9 +413,15 @@ Proof.
   iDestruct ("Hclo'" with "[$]") as "$".
 Qed.
 
-Lemma fupd_level_fupd E1 E2 P k : (|k={E1,E2}=> P) ⊢ |={E1,E2}=> P.
+Lemma fupd_level_le E1 E2 k1 k2 P : k1 ≤ k2 → (|k1={E1,E2}=> P) ⊢ |k2={E1,E2}=> P.
+Proof. rewrite ?uPred_fupd_level_eq => ?. apply fupd_split_level_le; naive_solver lia. Qed.
+
+Lemma fupd_level_split_level E1 E2 k1 mj k2 P : k1 ≤ k2 → (|k1={E1,E2}=> P) ⊢ |k2,mj={E1,E2}=> P.
+Proof. rewrite ?uPred_fupd_level_eq => ?. apply fupd_split_level_le; naive_solver lia. Qed.
+
+Lemma fupd_split_level_fupd E1 E2 P k mj : (|k,mj={E1,E2}=> P) ⊢ |={E1,E2}=> P.
 Proof.
-  rewrite ?uPred_fupd_level_eq /uPred_fupd_level_def.
+  rewrite ?uPred_fupd_split_level_eq /uPred_fupd_split_level_def.
   rewrite ?uPred_fupd_eq /uPred_fupd_def.
   rewrite ?ownE_op //.
   iIntros "HP (Hw&HAE&HE)".
@@ -155,70 +433,64 @@ Proof.
   iDestruct ("Hclo'" with "[$]") as "$".
 Qed.
 
-Lemma fupd_level_trans E1 E2 E3 k P : (|k={E1,E2}=> |k={E2,E3}=> P) ⊢ |k={E1,E3}=> P.
+Lemma fupd_level_fupd E1 E2 P k : (|k={E1,E2}=> P) ⊢ |={E1,E2}=> P.
+Proof. rewrite ?uPred_fupd_level_eq. apply fupd_split_level_fupd. Qed.
+
+Lemma fupd_split_level_trans E1 E2 E3 k mj P : (|k,mj={E1,E2}=> |k,mj={E2,E3}=> P) ⊢ |k,mj={E1,E3}=> P.
 Proof.
-  rewrite uPred_fupd_level_eq. iIntros "HP HwE".
+  rewrite uPred_fupd_split_level_eq. iIntros "HP HwE".
   iMod ("HP" with "HwE") as ">(Hw & HE & HP)". iApply "HP"; by iFrame.
 Qed.
 
-Lemma fupd_level_mask_frame_r' E1 E2 Ef k P:
-    E1 ## Ef → (|k={E1,E2}=> ⌜E2 ## Ef⌝ → P) ⊢ |k={E1 ∪ Ef,E2 ∪ Ef}=> P.
+Lemma fupd_level_trans E1 E2 E3 k P : (|k={E1,E2}=> |k={E2,E3}=> P) ⊢ |k={E1,E3}=> P.
+Proof. rewrite uPred_fupd_level_eq; apply fupd_split_level_trans. Qed.
+
+Lemma fupd_split_level_mask_frame_r' E1 E2 Ef k mj P:
+    E1 ## Ef → (|k,mj={E1,E2}=> ⌜E2 ## Ef⌝ → P) ⊢ |k,mj={E1 ∪ Ef,E2 ∪ Ef}=> P.
 Proof.
-  intros HE1Ef. rewrite uPred_fupd_level_eq /uPred_fupd_level_def ?ownE_op // ownE_op_MaybeEn //.
+  intros HE1Ef. rewrite uPred_fupd_split_level_eq /uPred_fupd_split_level_def ?ownE_op // ownE_op_MaybeEn //.
   iIntros "Hvs (Hw & HAE & HE1 & HEf)".
   iMod ("Hvs" with "[Hw HAE HE1]") as ">($ & (HAE & HE2) & HP)"; first by iFrame.
   iDestruct (ownE_op_MaybeEn' with "[HE2 HEf]") as "[? $]"; first by iFrame.
   iIntros "!> !>". iFrame. by iApply "HP".
 Qed.
 
+Lemma fupd_level_mask_frame_r' E1 E2 Ef k P:
+    E1 ## Ef → (|k={E1,E2}=> ⌜E2 ## Ef⌝ → P) ⊢ |k={E1 ∪ Ef,E2 ∪ Ef}=> P.
+Proof. rewrite uPred_fupd_level_eq; apply fupd_split_level_mask_frame_r'. Qed.
+
+Lemma fupd_split_level_frame_r E1 E2 k mj P R:
+  (|k,mj={E1,E2}=> P) ∗ R ⊢ |k,mj={E1,E2}=> P ∗ R.
+Proof. rewrite uPred_fupd_split_level_eq /uPred_fupd_split_level_def. by iIntros "[HwP $]". Qed.
+
 Lemma fupd_level_frame_r E1 E2 k P R:
   (|k={E1,E2}=> P) ∗ R ⊢ |k={E1,E2}=> P ∗ R.
-Proof.
-  rewrite uPred_fupd_level_eq /uPred_fupd_level_def. by iIntros "[HwP $]".
-Qed.
+Proof. rewrite uPred_fupd_level_eq; apply fupd_split_level_frame_r. Qed.
 
-(*
-Instance uPred_bi_fupd_level `{!invG Σ} : BiFUpd (uPredI (iResUR Σ)) :=
-  {| bi_fupd_mixin := uPred_fupd_level_mixin |}.
-
-Instance uPred_bi_bupd_fupd_level `{!invG Σ} : BiBUpdFUpd (uPredI (iResUR Σ)).
-Proof. rewrite /BiBUpdFupd_Level uPred_fupd_level_eq. by iIntros (E P) ">? [$ $] !> !>". Qed.
-*)
-
-(*
-Instance uPred_bi_fupd_level_plainly `{!invG Σ} : BiFUpdPlainly (uPredI (iResUR Σ)).
-Proof.
-  split.
-  - rewrite uPred_fupd_level_eq /uPred_fupd_level_def. iIntros (E P) "H [Hw HE]".
-    iAssert (◇ ■ P)%I as "#>HP".
-    { by iMod ("H" with "[$]") as "(_ & _ & HP)". }
-    by iFrame.
-  - rewrite uPred_fupd_level_eq /uPred_fupd_level_def. iIntros (E P Q) "[H HQ] [Hw HE]".
-    iAssert (◇ ■ P)%I as "#>HP".
-    { by iMod ("H" with "HQ [$]") as "(_ & _ & HP)". }
-    by iFrame.
-  - rewrite uPred_fupd_level_eq /uPred_fupd_level_def. iIntros (E P) "H [Hw HE]".
-    iAssert (▷ ◇ ■ P)%I as "#HP".
-    { iNext. by iMod ("H" with "[$]") as "(_ & _ & HP)". }
-    iFrame. iIntros "!> !> !>". by iMod "HP".
-  - rewrite uPred_fupd_level_eq /uPred_fupd_level_def. iIntros (E A Φ) "HΦ [Hw HE]".
-    iAssert (◇ ■ ∀ x : A, Φ x)%I as "#>HP".
-    { iIntros (x). by iMod ("HΦ" with "[$Hw $HE]") as "(_&_&?)". }
-    by iFrame.
-Qed.
-*)
+Global Instance fupd_split_level_proper E1 E2 k mj :
+  Proper ((≡) ==> (≡)) (uPred_fupd_split_level E1 E2 k mj) := ne_proper _.
 Global Instance fupd_level_proper E1 E2 k :
   Proper ((≡) ==> (≡)) (uPred_fupd_level E1 E2 k) := ne_proper _.
 
+
+Global Instance fupd_split_mono' E1 E2 k mj : Proper ((⊢) ==> (⊢)) (uPred_fupd_split_level E1 E2 k mj).
+Proof. intros P Q; apply fupd_split_level_mono. Qed.
 Global Instance fupd_mono' E1 E2 k : Proper ((⊢) ==> (⊢)) (uPred_fupd_level E1 E2 k).
 Proof. intros P Q; apply fupd_level_mono. Qed.
+Global Instance fupd_split_flip_mono' E1 E2 k mj :
+  Proper (flip (⊢) ==> flip (⊢)) (uPred_fupd_split_level E1 E2 k mj).
+Proof. intros P Q; apply fupd_split_level_mono. Qed.
 Global Instance fupd_flip_mono' E1 E2 k :
   Proper (flip (⊢) ==> flip (⊢)) (uPred_fupd_level E1 E2 k).
 Proof. intros P Q; apply fupd_level_mono. Qed.
 
+Lemma bupd_fupd_split_level E k mj P:
+  (|==> P) ⊢ |k,mj={E}=> P.
+Proof. rewrite uPred_fupd_split_level_eq. by iIntros ">? [$ $] !> !>". Qed.
+
 Lemma bupd_fupd_level E k P:
   (|==> P) ⊢ |k={E}=> P.
-Proof. rewrite uPred_fupd_level_eq. by iIntros ">? [$ $] !> !>". Qed.
+Proof. rewrite uPred_fupd_level_eq. apply bupd_fupd_split_level. Qed.
 
 Lemma fupd_level_intro E k P : P ⊢ |k={E}=> P.
 Proof. by rewrite {1}(fupd_level_intro_mask E E k P) // fupd_level_trans. Qed.
@@ -393,53 +665,161 @@ Proof. intros. by rewrite -(step_fupd_level_mask_mono Ei _ Ei _) // -!fupd_level
 
 End fupd_level.
 
-Section fupd_level.
+Section fupd_split_level.
 Context `{!invG Σ}.
-Implicit Types P: iProp Σ.
-Implicit Types E : coPset.
-Implicit Types k : nat.
+Lemma fupd_split_level_intro E k mj P : P ⊢ |k,mj={E}=> P.
+Proof. by rewrite {1}(fupd_split_level_intro_mask E E k mj P) // fupd_split_level_trans. Qed.
+Lemma fupd_split_level_intro_mask' E1 E2 k mj : E2 ⊆ E1 → ⊢@{iPropI Σ} |k,mj={E1,E2}=> |k,mj={E2,E1}=> emp.
+Proof. exact: fupd_split_level_intro_mask. Qed.
+Lemma fupd_split_level_except_0 E1 E2 k mj P : (|k,mj={E1,E2}=> ◇ P) ⊢ |k,mj={E1,E2}=> P.
+Proof. by rewrite {1}(fupd_split_level_intro E2 k mj P) except_0_fupd_split_level fupd_split_level_trans. Qed.
 
-Lemma fupd_level_plain_soundness `{!invPreG Σ} E1 E2 k (P: iProp Σ) `{!Plain P} :
-  (∀ `{Hinv: !invG Σ}, ⊢ |k={E1,E2}=> P) → ⊢ P.
+Global Instance from_assumption_fupd_split_level E k mj p P Q :
+  FromAssumption p P (|==> Q) → KnownRFromAssumption p P (|k,mj={E}=> Q)%I.
+Proof. rewrite /KnownRFromAssumption /FromAssumption=>->. apply bupd_fupd_split_level. Qed.
+
+Global Instance from_pure_fupd_split_level a E k mj P φ :
+  FromPure a P φ → FromPure a (|k,mj={E}=> P) φ.
+Proof. rewrite /FromPure. intros <-. apply fupd_split_level_intro. Qed.
+
+Lemma fupd_split_level_frame_l E1 E2 k mj R Q : (R ∗ |k,mj={E1,E2}=> Q) ⊢ |k,mj={E1,E2}=> R ∗ Q.
+Proof. rewrite !(comm _ R). apply fupd_split_level_frame_r. Qed.
+Lemma fupd_split_level_wand_l E1 E2 k mj P Q : (P -∗ Q) ∗ (|k,mj={E1,E2}=> P) ⊢ |k,mj={E1,E2}=> Q.
+Proof. by rewrite fupd_split_level_frame_l wand_elim_l. Qed.
+Lemma fupd_split_level_wand_r E1 E2 k mj P Q : (|k,mj={E1,E2}=> P) ∗ (P -∗ Q) ⊢ |k,mj={E1,E2}=> Q.
+Proof. by rewrite fupd_split_level_frame_r wand_elim_r. Qed.
+
+Lemma fupd_split_level_mask_weaken E1 E2 k mj P : E2 ⊆ E1 → P ⊢ |k,mj={E1,E2}=> P.
 Proof.
-  iIntros (Hfupd_level). apply (later_soundness _); simpl.
-   iMod wsat_alloc as (Hinv) "[Hw HE]".
-  iAssert (|k={⊤,E2}=> P)%I as "H".
-  { iMod (fupd_level_intro_mask'); last iApply Hfupd_level. done. }
-  rewrite uPred_fupd_level_eq /uPred_fupd_level_def.
-  iMod ("H" with "[$Hw HE]") as "[Hw [HE >H']]"; iFrame.
-  iApply (ownE_weaken with "HE"). set_solver.
+  intros ?. rewrite -{1}(right_id emp%I bi_sep P%I).
+  rewrite (fupd_split_level_intro_mask E1 E2 k mj emp%I) //.
+  by rewrite fupd_split_level_frame_l sep_elim_l.
+Qed.
+
+Lemma fupd_split_level_mask_frame_r E1 E2 k mj Ef P :
+  E1 ## Ef → (|k,mj={E1,E2}=> P) ⊢ |k,mj={E1 ∪ Ef,E2 ∪ Ef}=> P.
+Proof.
+  intros ?. rewrite -fupd_split_level_mask_frame_r' //. f_equiv.
+  apply impl_intro_l, and_elim_r.
+Qed.
+Lemma fupd_split_level_mask_mono E1 E2 k mj P : E1 ⊆ E2 → (|k,mj={E1}=> P) ⊢ |k,mj={E2}=> P.
+Proof.
+  intros (Ef&->&?)%subseteq_disjoint_union_L. by apply fupd_split_level_mask_frame_r.
+Qed.
+
+Lemma fupd_split_level_sep E k mj P Q : (|k,mj={E}=> P) ∗ (|k,mj={E}=> Q) ⊢ |k,mj={E}=> P ∗ Q.
+Proof. by rewrite fupd_split_level_frame_r fupd_split_level_frame_l fupd_split_level_trans. Qed.
+Lemma fupd_split_level_mask_frame E E' E1 E2 k mj P :
+  E1 ⊆ E →
+  (|k,mj={E1,E2}=> |k,mj={E2 ∪ (E ∖ E1),E'}=> P) -∗ (|k,mj={E,E'}=> P).
+Proof.
+  intros ?. rewrite (fupd_split_level_mask_frame_r _ _ _ _ (E ∖ E1)); last set_solver.
+  rewrite fupd_split_level_trans.
+  by replace (E1 ∪ E ∖ E1) with E by (by apply union_difference_L).
+Qed.
+
+Global Instance into_wand_fupd_split_level E k mj p q R P Q :
+  IntoWand false false R P Q →
+  IntoWand p q (|k,mj={E}=> R) (|k,mj={E}=> P) (|k,mj={E}=> Q).
+Proof.
+  rewrite /IntoWand /= => HR. rewrite !intuitionistically_if_elim HR.
+  apply wand_intro_l. by rewrite fupd_split_level_sep wand_elim_r.
+Qed.
+
+Global Instance into_wand_fupd_split_level_persistent E1 E2 k mj p q R P Q :
+  IntoWand false q R P Q → IntoWand p q (|k,mj={E1,E2}=> R) P (|k,mj={E1,E2}=> Q).
+Proof.
+  rewrite /IntoWand /= => HR. rewrite intuitionistically_if_elim HR.
+  apply wand_intro_l. by rewrite fupd_split_level_frame_l wand_elim_r.
+Qed.
+
+Global Instance into_wand_fupd_split_level_args E1 E2 k mj p q R P Q :
+  IntoWand p false R P Q → IntoWand' p q R (|k,mj={E1,E2}=> P) (|k,mj={E1,E2}=> Q).
+Proof.
+  rewrite /IntoWand' /IntoWand /= => ->.
+  apply wand_intro_l. by rewrite intuitionistically_if_elim fupd_split_level_wand_r.
+Qed.
+
+Global Instance from_sep_fupd_split_level E k mj P Q1 Q2 :
+  FromSep P Q1 Q2 → FromSep (|k,mj={E}=> P) (|k,mj={E}=> Q1) (|k,mj={E}=> Q2).
+Proof. rewrite /FromSep =><-. apply fupd_split_level_sep. Qed.
+
+Global Instance from_or_fupd_split_level E1 E2 k mj P Q1 Q2 :
+  FromOr P Q1 Q2 → FromOr (|k,mj={E1,E2}=> P) (|k,mj={E1,E2}=> Q1) (|k,mj={E1,E2}=> Q2).
+  rewrite /FromOr=><-. apply or_elim; apply fupd_split_level_mono;
+                         [apply bi.or_intro_l|apply bi.or_intro_r].
+Qed.
+
+Global Instance from_exist_fupd_split_level {A} E1 k mj E2 P (Φ : A → iProp Σ) :
+  FromExist P Φ → FromExist (|k,mj={E1,E2}=> P) (λ a, |k,mj={E1,E2}=> Φ a)%I.
+Proof.
+  rewrite /FromExist=><-. apply exist_elim=> a. by rewrite -(exist_intro a).
 Qed.
 
 (*
-Lemma step_fupd_levelN_soundness `{!invPreG Σ} φ n :
-  (∀ `{Hinv: !invG Σ}, ⊢@{iPropI Σ} |={⊤}[∅]▷=>^n |={⊤,∅}=> ⌜ φ ⌝) →
-  φ.
+Global Instance from_forall_fupd_split_level E1 E2 k mj {A} P (Φ : A → iProp Σ) :
+  (* Some cases in which [E2 ⊆ E1] holds *)
+  TCOr (TCEq E1 E2) (TCOr (TCEq E1 ⊤) (TCEq E2 ∅)) →
+  FromForall P Φ → (∀ x, Plain (Φ x)) →
+  FromForall (|k,mj={E1,E2}=> P)%I (λ a, |k,mj={E1,E2}=> (Φ a))%I.
 Proof.
-  intros Hiter.
-  apply (soundness (M:=iResUR Σ) _  (S n)); simpl.
-  apply (fupd_level_plain_soundness ⊤ ⊤ _)=> Hinv.
-  iPoseProof (Hiter Hinv) as "H". clear Hiter.
-  destruct n as [|n].
-  - iApply fupd_level_plainly_mask_empty. iMod "H" as %?; auto.
-  - iDestruct (step_fupd_levelN_wand _ _ _ _ (|={⊤}=> ⌜φ⌝)%I with "H []") as "H'".
-    { by iApply fupd_level_plain_mask_empty. }
-    rewrite -step_fupd_levelN_S_fupd_level.
-    iMod (step_fupd_levelN_plain with "H'") as "Hφ". iModIntro. iNext.
-    rewrite -later_laterN laterN_later.
-    iNext. by iMod "Hφ".
+  rewrite /FromForall=> -[->|[->|->]] <- ?; rewrite fupd_plain_forall; set_solver.
+Qed.
+*)
+
+Global Instance except_0_fupd_split_level' E1 E2 k mj P :
+  IsExcept0 (|k,mj={E1,E2}=> P).
+Proof. by rewrite /IsExcept0 except_0_fupd_split_level. Qed.
+
+Global Instance from_modal_fupd_split_level E k mj P :
+  FromModal modality_id (|k,mj={E}=> P) (|k,mj={E}=> P) P.
+Proof. by rewrite /FromModal /= -fupd_split_level_intro. Qed.
+
+Global Instance elim_modal_bupd_fupd_split_level p E1 E2 k mj P Q :
+  ElimModal True p false (|==> P) P (|k,mj={E1,E2}=> Q) (|k,mj={E1,E2}=> Q) | 10.
+Proof.
+  by rewrite /ElimModal intuitionistically_if_elim
+    (bupd_fupd_split_level E1 k mj) fupd_split_level_frame_r wand_elim_r fupd_split_level_trans.
+Qed.
+Global Instance elim_modal_fupd_split_level_fupd_split_level p E1 E2 E3 k mj P Q :
+  ElimModal True p false (|k,mj={E1,E2}=> P) P (|k,mj={E1,E3}=> Q) (|k,mj={E2,E3}=> Q).
+Proof.
+  by rewrite /ElimModal intuitionistically_if_elim
+    fupd_split_level_frame_r wand_elim_r fupd_split_level_trans.
+Qed.
+(*
+Global Instance elim_modal_fupd_fupd_split_level p E1 E2 k mj P Q :
+  ElimModal True p false (|={E1,E2}=> P) P (|(S k)={E1,E3}=> Q) (|(S k)={E2,E3}=> Q).
+Proof.
+  rewrite /ElimModal => ??. rewrite (fupd_fupd_split_level _ _ k) intuitionistically_if_elim
+    fupd_split_level_frame_r wand_elim_r fupd_split_level_trans //=.
+Qed.
+*)
+
+Global Instance elim_acc_fupd_split_level {X} E1 E2 E k mj α β mγ Q :
+  ElimAcc (X:=X) (uPred_fupd_split_level E1 E2 k mj) (uPred_fupd_split_level E2 E1 k mj) α β mγ
+          (|k,mj={E1,E}=> Q)
+          (λ x, |k,mj={E2}=> β x ∗ (mγ x -∗? |k,mj={E1,E}=> Q))%I.
+Proof.
+  rewrite /ElimAcc.
+  iIntros "Hinner >Hacc". iDestruct "Hacc" as (x) "[Hα Hclose]".
+  iMod ("Hinner" with "Hα") as "[Hβ Hfin]".
+  iMod ("Hclose" with "Hβ") as "Hγ". by iApply "Hfin".
 Qed.
 
-Lemma step_fupd_levelN_soundness' `{!invPreG Σ} φ n :
-  (∀ `{Hinv: !invG Σ}, ⊢@{iPropI Σ} |={⊤}[∅]▷=>^n ⌜ φ ⌝) →
-  φ.
+Global Instance frame_fupd_split_level p E1 E2 k mj R P Q :
+  Frame p R P Q → Frame p R (|k,mj={E1,E2}=> P) (|k,mj={E1,E2}=> Q).
+Proof. rewrite /Frame=><-. by rewrite fupd_split_level_frame_l. Qed.
+
+Lemma fupd_split_level_mask_mono' E1 E2 E1' E2' k mj P : E1 ⊆ E2 → E2' ⊆ E1' → (|k,mj={E1, E1'}=> P) ⊢ |k,mj={E2,E2'}=> P.
 Proof.
-  iIntros (Hiter). eapply (step_fupd_levelN_soundness _ n).
-  iIntros (Hinv). iPoseProof (Hiter Hinv) as "Hiter".
-  iApply (step_fupd_levelN_wand with "Hiter"). by iApply fupd_level_mask_weaken.
+  iIntros (??) "H".
+  iMod (fupd_split_level_intro_mask' _ E1) as "Hclo"; auto.
+  iMod "H".
+  iApply (fupd_split_level_mask_weaken); auto.
 Qed.
- *)
-End fupd_level.
+
+End fupd_split_level.
 
 Section schema_test_fupd.
 Context `{!invG Σ}.
@@ -455,14 +835,14 @@ Definition bi_sch_bupd_wand (P1 P2: bi_schema) :=
 
 Definition bi_sch_fupd E1 E2 (P: bi_schema) : bi_schema :=
   bi_sch_bupd_wand
-    (bi_sch_sep (bi_sch_wsat) (bi_sch_ownE (λ k, AE k ∪ MaybeEn E1)))
+    (bi_sch_sep (bi_sch_wsat) (bi_sch_ownE (λ k, AE k (Some O) ∪ MaybeEn E1)))
     (bi_sch_except_0 (bi_sch_sep (bi_sch_wsat)
-                                (bi_sch_sep (bi_sch_ownE (λ k, AE k ∪ MaybeEn E2)) P))).
+                                (bi_sch_sep (bi_sch_ownE (λ k, AE k (Some O) ∪ MaybeEn E2)) P))).
 
 Lemma bi_sch_fupd_interp' E1 E2 lvl Qs Qs_mut Psch P:
   bi_schema_interp lvl Qs Qs_mut Psch = P →
   bi_schema_interp lvl Qs Qs_mut (bi_sch_fupd E1 E2 Psch) =
-    (wsat lvl ∗ ownE (AE lvl ∪ MaybeEn E1) ==∗ ◇ (wsat lvl ∗ ownE (AE lvl ∪ MaybeEn E2) ∗ P))%I.
+    (wsat lvl ∗ ownE (AE lvl (Some 0) ∪ MaybeEn E1) ==∗ ◇ (wsat lvl ∗ ownE (AE lvl (Some 0) ∪ MaybeEn E2) ∗ P))%I.
 Proof.
   intros Heq.
   rewrite ?bi_schema_interp_unfold //=.
@@ -473,9 +853,9 @@ Qed.
 Lemma bi_sch_fupd_interp E1 E2 lvl Qs Qs_mut Psch P:
   bi_schema_interp (S lvl) Qs Qs_mut Psch = P →
   bi_schema_interp (S lvl) Qs Qs_mut (bi_sch_fupd E1 E2 Psch) =
-  (|lvl={E1, E2}=> P)%I.
+  (|lvl,(Some 0)={E1, E2}=> P)%I.
 Proof.
-  intros Heq. rewrite uPred_fupd_level_eq /uPred_fupd_level_def. by apply bi_sch_fupd_interp'.
+  intros Heq. rewrite uPred_fupd_split_level_eq. by apply bi_sch_fupd_interp'.
 Qed.
 
 End schema_test_fupd.
